#trigonometrie #analyse 
$\forall x \in \mathbb{R}, \; ch^{2}(x)-sh^{2}(x)=1$ 
## Cosinus hyperbolique
$\displaystyle  ch: \mathbb{R} \longrightarrow \mathbb{R}; \quad  ch(x)=\frac{e^{x}+e^{-x}}{2}$ 
- $ch'(x)=sh(x)$ 
- $\forall x \in \mathbb{R}, \; ch(-x)=ch(x)$ 

| ![[image tableau ch.png\|300]] | ![[image graphique ch.png\|300]] |
| ------------------------------ | -------------------------------- |
|                                |                                  |

## Sinus hyperbolique 
$\displaystyle sh: \mathbb{R} \longrightarrow \mathbb{R}; \quad  sh(x)=\frac{e^{x}-e^{-x}}{2}$ 
- $sh'(x)=ch(x)$ 
- $\forall x \in \mathbb{R}, \; sh(-x)=sh(x)$ 

| ![[image tableau sh.png\|300]] | ![[image graphique sh.png\|200]] |
| ------------------------------ | -------------------------------- |
|                                |                                  |







 
