- $\displaystyle (1+x)^{\alpha }= 1+\alpha x + \frac{\alpha (\alpha -1)}{2!}x^{2}+ \frac{\alpha (\alpha -1)(\alpha -2)}{3!}x^{3} + x^{3}\varepsilon(x)$ 
- $\displaystyle e^{x}= 1+x+ \frac{x^{2}}{2!}+ \frac{x^{3}}{3!} + x^{3}\varepsilon(x)$
- $\displaystyle \frac{1}{1-x} = 1+x+x^{2}+x^{3}+x^{3} \varepsilon (x)$ 
- $\displaystyle \ln(1+x) = x - \frac{x^{2}}{2}+ \frac{x^{3}}{3} + x^{3} \varepsilon(x)$ 
- $\displaystyle \sin(x) = x- \frac{x^{3}}{3!}+ x^{3}\varepsilon(x)$ 
- $\displaystyle \cos(x)= 1 - \frac{x^{2}}{2!} + x^{3}\varepsilon(x)$ 
- $\displaystyle sh(x) = x + \frac{x^{3}}{3!} + x^{3}\varepsilon (x)$ 
- $\displaystyle ch(x)= 1 + \frac{x^{2}}{2!} + x^{3}\varepsilon(x)$ 
- $\displaystyle \arctan(x) = x - \frac{x^{3}}{3}+o(x^{3})$ 
- $\displaystyle \tan(x)=x+ \frac{x^{3}}{3} + o(x^{3})$
